added make_honest function and a lemma documenting what can and cannot be proven

examples/crypto/cryptobox/Box.Indexing.fst
@@ -8,8 +8,6 @@ open FStar.HyperStack
 module MR = FStar.Monotonic.RRef
 module MM = MonotoneMap
 
-
-// This should be UInt32?
 type id = int
 assume Index_hasEq: hasEq id
 type range = fun id -> bool
@@ -20,17 +18,17 @@ val id_table_region: (r:MR.rid{color r = id_table_color /\ extends r root /\ is_
 let id_table_region = new_colored_region root id_table_color
 
 
-//val id_table: MM.t
+val id_table: MM.t id_table_region id range inv
 let id_table = MM.alloc #id_table_region #id #range #inv 
 
-
-//abstract type val honest: i:id -> Tot bool
 type honest (i:id) =
   MR.witnessed (MM.contains id_table i true)
 
 type dishonest (i:id) =
   MR.witnessed (MM.contains id_table i false)
 
+type fixed (i:id) =
+  MR.witnessed (MM.defined id_table i)
 
 val make_dishonest: (i:id) -> ST (unit)
   (requires (fun h0 -> MM.fresh id_table i h0))
@@ -39,20 +37,26 @@ let make_dishonest i =
   MM.extend id_table i false;
   ()
 
-val honestST: i:id -> ST(b:bool{(b ==> honest i) /\ (not b ==> dishonest i)})
+val make_honest: (i:id) -> ST (unit)
+  (requires (fun h0 -> MM.fresh id_table i h0))
+  (ensures (fun h0 _ h1 -> honest i))
+let make_honest i =
+  MM.extend id_table i true;
+  ()
+  
+
+val honestST: i:id{fixed i} -> ST(b:bool{(b ==> honest i) /\ (not b ==> dishonest i)})
   (requires (fun h0 -> True))
   (ensures (fun h0 b h1 ->
-    modifies_one id_table_region h0 h1 
+    modifies_none h0 h1 
     /\ MR.m_contains id_table h1
   ))
-let honestST (i:id) =
+let honestST i =
   MR.m_recall id_table;
+  MR.testify(MM.defined id_table i);
   match MM.lookup id_table i with
   |Some v -> 
     v
-  |None -> 
-    MM.extend id_table i true;
-    true
 
 abstract type ae_id = 
   | AE_id: i:(id*id){fst i <= snd i} -> ae_id
@@ -70,21 +74,35 @@ val unique_id_generation: i1:id -> i2:id -> Lemma
   [SMTPat (generate_ae_id i1 i2)]
 let unique_id_generation i1 i2 = ()
 
+val honest_dishonest_lemma: i:id -> ST(unit)
+  (requires (fun h -> fixed i))
+  (ensures (fun h0 _ h1 -> modifies_none h0 h1 /\
+    ( dishonest i \/ honest i ) /\
+    ( ~(honest i) ==> dishonest i ) /\
+    ( ~(dishonest i) ==> honest i ) /\
+//    ( honest i ==> ~(dishonest i) ) /\ //This cannot be proven.
+    True
+  ))
+let honest_dishonest_lemma i = 
+  let h = get() in
+  MR.testify (MM.defined id_table i); 
+  match MM.lookup id_table i with
+  |Some v ->  MR.testify(MM.contains id_table i v); ()
 
-//val ae_honest: (k_i:ae_id) -> Tot Type0 //(t:Type{t ==> honest (fst k_i.i) /\ honest (snd k_i.i)})
 type ae_honest k_i =
   honest (fst k_i.i) /\ honest (snd k_i.i)
-
 
 type ae_dishonest (k_i:ae_id) =
   dishonest (fst k_i.i) \/ dishonest (snd k_i.i)
 
-val ae_honestST: k_i:ae_id -> ST(b:bool{(b ==> (ae_honest k_i)) /\ (not b ==> (ae_dishonest k_i))})
+type ae_fixed (k_i:ae_id) = 
+  fixed (fst k_i.i) /\ fixed(snd k_i.i)
+
+val ae_honestST: k_i:ae_id{ae_fixed k_i} -> ST(b:bool{(b ==> (ae_honest k_i)) /\ (not b ==> (ae_dishonest k_i))})
   (requires (fun h0 -> True))
   (ensures (fun h0 b h1 ->
-    modifies_one id_table_region h0 h1 
+    modifies_none h0 h1
     /\ MR.m_contains id_table h1
-    ///\ MR.m_sel h1 id_table == snoc (MR.m_sel h0 id_table) i
   ))
 let ae_honestST k_i =
   let h1 = honestST (fst k_i.i) in 
